Proved reducibility of internal actions with weaker conditions.

src/Commutable.v
@@ -6,43 +6,7 @@ Set Implicit Arguments.
 
 Open Scope list.
 
-(* Definition ruleOfL {MsgT} (lbl: RLabel MsgT): option Rule := *)
-(*   match lbl with *)
-(*   | RlblInt rule _ _ => Some rule *)
-(*   | _ => None *)
-(*   end. *)
-
-(* Fixpoint rulesOfH (hst: MHistory) := *)
-(*   match hst with *)
-(*   | nil => nil *)
-(*   | lbl :: hst' => (ruleOfL lbl) ::> (rulesOfH hst') *)
-(*   end. *)
-
-(* Definition insOfL {MsgT} (lbl: RLabel MsgT): list (Id MsgT) := *)
-(*   match lbl with *)
-(*   | RlblInt _ ins _ => ins *)
-(*   | RlblOuts outs => outs *)
-(*   | _ => nil *)
-(*   end. *)
-
-(* Definition outsOfL {MsgT} (lbl: RLabel MsgT): list (Id MsgT) := *)
-(*   match lbl with *)
-(*   | RlblIns ins => ins *)
-(*   | RlblInt _ _ outs => outs *)
-(*   | _ => nil *)
-(*   end. *)
-
-(* Fixpoint insOfH (hst: MHistory) := *)
-(*   match hst with *)
-(*   | nil => nil *)
-(*   | lbl :: hst' => insOfH hst' ++ insOfL lbl *)
-(*   end. *)
-
-(* Fixpoint outsOfH (hst: MHistory) := *)
-(*   match hst with *)
-(*   | nil => nil *)
-(*   | lbl :: hst' => outsOfH hst' ++ outsOfL lbl *)
-(*   end. *)
+(*! Reducibility (commutativity) of internal state transitions *)
 
 (** TODO: need to check whether the disjointness between [ins1] and [ins2] 
  * (or [outs1] and [outs2]) is required. *)
@@ -51,40 +15,261 @@ Definition NonConflictingR {ifc: OStateIfc} (rule1 rule2: Rule ifc) :=
     rule_precond rule1 post1 porq1 ins1 ->
     rule_trs rule1 post1 porq1 ins1 = (nost1, norq1, outs1) ->
     rule_precond rule2 nost1 norq1 ins2 ->
-    (* 1) Precondition of [rule2] holds if the one of [rule1] holds. *)
+    (* 1) Preconditions of [rule2] hold if the ones of [rule1] hold. *)
     rule_precond rule2 post1 porq1 ins2 /\
-    forall nost2 norq2 outs2,
-      rule_trs rule2 post1 porq1 ins2 = (nost2, norq2, outs2) ->
-      (* 2) Precondition of [rule1] holds after a transition by [rule2]. *)
-      rule_precond rule1 nost2 norq2 ins1 /\
-      (* 3) Transitions by [rule1; rule2] and [rule2; rule1] are same. *)
-      fst (rule_trs rule2 nost1 norq1 ins2) =
-      fst (rule_trs rule1 nost2 norq2 ins1).
+    idsOf ins2 = rule_msgs_from rule2 porq1 /\
+    let (no2, outs2) := rule_trs rule2 nost1 norq1 ins2 in
+    let (nost2, norq2) := no2 in
+    let (rno2, routs2) := rule_trs rule2 post1 porq1 ins2 in
+    let (rnost2, rnorq2) := rno2 in
+    let (rno1, routs1) := rule_trs rule1 rnost2 rnorq2 ins1 in
+    let (rnost1, rnorq1) := rno1 in
+    (* ?? *)
+    routs2 = outs2 /\
+    (* 2) Precondition of [rule1] holds after a transition by [rule2]. *)
+    rule_precond rule1 rnost2 rnorq2 ins1 /\
+    idsOf ins1 = rule_msgs_from rule1 rnorq2 /\
+    (* 3) Transitions by [rule1; rule2] and [rule2; rule1] are same. *)
+    no2 = rno1 /\ outs1 = routs1.
+
+Definition NonConflictingL (sys: System)
+           (oidx1 ridx1 oidx2 ridx2: IdxT) :=
+  oidx1 <> oidx2 \/
+  (oidx1 = oidx2 /\
+   forall obj rule1 rule2,
+     In obj (sys_objs sys) -> obj_idx obj = oidx1 ->
+     In rule1 (obj_rules obj) -> rule_idx rule1 = ridx1 ->
+     In rule2 (obj_rules obj) -> rule_idx rule2 = ridx2 ->
+     NonConflictingR rule1 rule2).
 
 Definition NonConflicting (sys: System) (hst1 hst2: MHistory) :=
-  forall obj rule1 rule2 ins1 outs1 ins2 outs2,
-    In obj (sys_objs sys) ->
-    In rule1 (obj_rules obj) ->
-    In rule2 (obj_rules obj) ->
-    In (RlblInt (obj_idx obj) (rule_idx rule1) ins1 outs1) hst1 ->
-    In (RlblInt (obj_idx obj) (rule_idx rule2) ins2 outs2) hst2 ->
-    NonConflictingR rule1 rule2.
+  forall oidx1 ridx1 ins1 outs1 oidx2 ridx2 ins2 outs2,
+    In (RlblInt oidx1 ridx1 ins1 outs1) hst1 ->
+    In (RlblInt oidx2 ridx2 ins2 outs2) hst2 ->
+    NonConflictingL sys oidx1 ridx1 oidx2 ridx2.
 
 Definition Discontinuous (sys: System) (hst1 hst2: MHistory) :=
-  forall inits1 ins1 outs1 eouts1 inits2 ins2 outs2 eouts2,
+  exists inits1 ins1 outs1 eouts1 inits2 ins2 outs2 eouts2,
     Atomic msg_dec inits1 ins1 hst1 outs1 eouts1 /\
     Atomic msg_dec inits2 ins2 hst2 outs2 eouts2 /\
     DisjList (idsOf ins1) (idsOf ins2) /\
-    DisjList inits1 eouts2 /\
+    DisjList outs1 inits2 /\
     DisjList (idsOf outs1) (idsOf outs2).
 
+Lemma nonconflicting_head_1:
+  forall sys lbl1 hst1 hst2,
+    NonConflicting sys (lbl1 :: hst1) hst2 ->
+    NonConflicting sys [lbl1] hst2.
+Proof.
+  unfold NonConflicting; intros.
+  Common.dest_in.
+  eapply H; eauto.
+  left; eauto.
+Qed.
+
+Lemma nonconflicting_head_2:
+  forall sys hst1 lbl2 hst2,
+    NonConflicting sys hst1 (lbl2 :: hst2) ->
+    NonConflicting sys hst1 [lbl2].
+Proof.
+  unfold NonConflicting; intros.
+  Common.dest_in.
+  eapply H; eauto.
+  left; eauto.
+Qed.
+
+Lemma nonconflicting_tail_1:
+  forall sys lbl1 hst1 hst2,
+    NonConflicting sys (lbl1 :: hst1) hst2 ->
+    NonConflicting sys hst1 hst2.
+Proof.
+  unfold NonConflicting; intros.
+  eapply H; eauto.
+  right; eauto.
+Qed.
+
+Lemma nonconflicting_tail_2:
+  forall sys hst1 lbl2 hst2,
+    NonConflicting sys hst1 (lbl2 :: hst2) ->
+    NonConflicting sys hst1 hst2.
+Proof.
+  unfold NonConflicting; intros.
+  eapply H; eauto.
+  right; eauto.
+Qed.
+
+Lemma msg_int_commutes:
+  forall sys oidx1 ridx1 ins1 outs1 oidx2 ridx2 ins2 outs2,
+    NonConflictingL sys oidx1 ridx1 oidx2 ridx2 ->
+    DisjList (idsOf ins1) (idsOf ins2) ->
+    DisjList outs1 ins2 ->
+    DisjList (idsOf outs1) (idsOf outs2) ->
+    Reducible sys [RlblInt oidx2 ridx2 ins2 outs2; RlblInt oidx1 ridx1 ins1 outs1]
+              [RlblInt oidx1 ridx1 ins1 outs1; RlblInt oidx2 ridx2 ins2 outs2].
+Proof.
+  unfold Reducible; intros.
+  dest_steps; dest_step_m.
+
+  destruct H; dest.
+  - econstructor.
+    + econstructor.
+      * econstructor.
+      * econstructor; try reflexivity; try eassumption.
+        { mred. }
+        { mred. }
+        { eapply FirstMPI_Forall_deqMsgs.
+          { apply DisjList_comm; eassumption. }
+          { eapply FirstMPI_Forall_enqMsgs_inv.
+            { apply DisjList_comm; eassumption. }
+            { assumption. }
+          }
+        }
+    + econstructor; try reflexivity; try eassumption.
+      * mred.
+      * mred.
+      * apply FirstMPI_Forall_enqMsgs.
+        apply FirstMPI_Forall_deqMsgs; auto.
+      * f_equal.
+        { meq. }
+        { meq. }
+        { rewrite <-enqMsgs_deqMsgs_FirstMPI_comm.
+          { rewrite deqMsgs_deqMsgs_comm by (apply DisjList_comm; assumption).
+            rewrite enqMsgs_enqMsgs_comm with (msgs1:= outs2)
+              by (apply DisjList_comm; assumption).
+            rewrite enqMsgs_deqMsgs_FirstMPI_comm with (msgs2:= outs2).
+            { reflexivity. }
+            { destruct H15; auto. }
+            { apply FirstMPI_Forall_deqMsgs; auto. }
+          }
+          { destruct H26; auto. }
+          { eapply FirstMPI_Forall_enqMsgs_inv.
+            { apply DisjList_comm; eassumption. }
+            { assumption. }
+          }
+        }
+
+  - assert (obj = obj0) by (eapply obj_same_id_in_system_same; eauto).
+    subst; mred; simpl in *.
+    specialize (H3 _ _ _ H7 eq_refl H8 eq_refl H11 eq_refl).
+
+    red in H3.
+    pose proof (UIP_refl _ _ Hifc0); subst.
+    specialize (H3 _ _ _ _ _ _ _ H18 H19 H29); dest.
+
+    remember (rule_trs rule0 pos porq0 ins2) as trs2.
+    destruct trs2 as [[tnost2 tnorq2] touts2]; inv H30.
+    remember (rule_trs rule0
+                       match Hifc in (_ = o) return (OState o) with
+                       | eq_refl => ost_st os
+                       end porq ins2) as rtrs2.
+    destruct rtrs2 as [[rnost2 rnorq2] routs2]; dest; subst.
+    remember (rule_trs rule rnost2 rnorq2 ins1) as rtrs1.
+    destruct rtrs1 as [[rnost1 rnorq1] routs1]; dest; subst.
+    
+    econstructor.
+    + econstructor.
+      * econstructor.
+      * econstructor; try reflexivity; try eassumption.
+        { eapply FirstMPI_Forall_deqMsgs.
+          { apply DisjList_comm; eassumption. }
+          { eapply FirstMPI_Forall_enqMsgs_inv.
+            { apply DisjList_comm; eassumption. }
+            { eassumption. }
+          }
+        }
+        { apply eq_sym; eassumption. }
+    + econstructor.
+      * assumption.
+      * assumption.
+      * reflexivity.
+      * instantiate (2:= (oss+[obj_idx obj0 <- {| ost_st := rnost2 |}])%fmap).
+        mred.
+      * instantiate (2:= (orqs+[obj_idx obj0 <- rnorq2])%fmap).
+        mred.
+      * instantiate (1:= enqMsgs outs2 (deqMsgs (idsOf ins2) msgs)).
+        apply FirstMPI_Forall_enqMsgs.
+        apply FirstMPI_Forall_deqMsgs; auto.
+      * assumption.
+      * assumption.
+      * assumption.
+      * instantiate (1:= eq_refl); simpl.
+        assumption.
+      * simpl; apply eq_sym; eassumption.
+      * assumption.
+      * assumption.
+      * reflexivity.
+      * inv H20; f_equal.
+        { meq. }
+        { meq. }
+        { rewrite <-enqMsgs_deqMsgs_FirstMPI_comm.
+          { rewrite deqMsgs_deqMsgs_comm by (apply DisjList_comm; assumption).
+            rewrite enqMsgs_enqMsgs_comm with (msgs1:= outs2)
+              by (apply DisjList_comm; assumption).
+            rewrite enqMsgs_deqMsgs_FirstMPI_comm with (msgs2:= outs2).
+            { reflexivity. }
+            { destruct H15; auto. }
+            { apply FirstMPI_Forall_deqMsgs; auto. }
+          }
+          { destruct H26; auto. }
+          { eapply FirstMPI_Forall_enqMsgs_inv.
+            { apply DisjList_comm; eassumption. }
+            { assumption. }
+          }
+        }
+Qed.
+
+Lemma nonconflicting_discontinuous_commutable_atomic_0:
+  forall sys oidx1 ridx1 mins1 mouts1 inits2 ins2 hst2 outs2 eouts2,
+    Atomic msg_dec inits2 ins2 hst2 outs2 eouts2 ->
+    NonConflicting sys [RlblInt oidx1 ridx1 mins1 mouts1] hst2 ->
+    DisjList (idsOf mins1) (idsOf ins2) ->
+    DisjList mouts1 inits2 ->
+    DisjList (idsOf mouts1) (idsOf outs2) ->
+    Reducible sys (hst2 ++ [RlblInt oidx1 ridx1 mins1 mouts1])
+              (RlblInt oidx1 ridx1 mins1 mouts1 :: hst2).
+Proof.
+  induction 1; simpl; intros.
+
+  - apply msg_int_commutes; auto.
+    
+Admitted.
+  
 Lemma nonconflicting_discontinuous_commutable_atomic:
   forall sys hst1 hst2,
     NonConflicting sys hst1 hst2 ->
     Discontinuous sys hst1 hst2 ->
     Reducible sys (hst2 ++ hst1) (hst1 ++ hst2).
 Proof.
-Admitted.
+  unfold Discontinuous; intros.
+  destruct H0 as [inits1 [ins1 [outs1 [eouts1 [inits2 [ins2 [outs2 [eouts2 ?]]]]]]]].
+  dest.
+
+  induction H0; simpl; intros; subst;
+    [eapply nonconflicting_discontinuous_commutable_atomic_0; eauto|].
+
+  replace (hst2 ++ RlblInt oidx ridx rins routs :: hst)
+    with ((hst2 ++ [RlblInt oidx ridx rins routs]) ++ hst)
+    by (rewrite <-app_assoc; reflexivity).
+ 
+  eapply reducible_trans.
+  - apply reducible_app_2.
+    eapply nonconflicting_discontinuous_commutable_atomic_0;
+      try (eapply H1; eauto).
+    + eapply nonconflicting_head_1; eauto.
+    + rewrite idsOf_app in H2.
+      apply DisjList_app_3 in H2; dest; auto.
+    + apply DisjList_app_3 in H3; dest; auto.
+    + rewrite idsOf_app in H4.
+      apply DisjList_app_3 in H4; dest; auto.
+  - simpl; apply reducible_cons.
+    apply IHAtomic; auto.
+    + eapply nonconflicting_tail_1; eauto.
+    + rewrite idsOf_app in H2.
+      apply DisjList_app_3 in H2; dest; auto.
+    + apply DisjList_app_3 in H3; dest; auto.
+    + rewrite idsOf_app in H4.
+      apply DisjList_app_3 in H4; dest; auto.
+Qed.
 
 Close Scope list.
 
